Apply Markus' suggestion

src/Std/Data/Internal/List/Associative.lean
@@ -5349,13 +5349,13 @@ theorem getKey?_filter_containsKey_of_containsKey_right [BEq α] [EquivBEq α]
   · exact dl₁
 
 /-- Internal implementation detail of the hash map -/
-def eraseList [BEq α] (l toErase : List ((a : α) × β a)) : List ((a : α) × β a) :=
+def eraseList [BEq α] (l : List ((a : α) × β a))  (toErase : List α): List ((a : α) × β a) :=
   match toErase with
   | .nil => l
-  | .cons ⟨k, _⟩ toErase => eraseList (eraseKey k l) toErase
+  | .cons k toErase => eraseList (eraseKey k l) toErase
 
 theorem eraseList_perm_filter_containsKey [BEq α] [EquivBEq α] (l toErase : List ((a : α) × β a)) (hl : DistinctKeys l):
-    List.Perm (eraseList l toErase) (l.filter (fun p => !containsKey p.fst toErase)) := by
+    List.Perm (eraseList l (toErase.map (·.1))) (l.filter (fun p => !containsKey p.fst toErase)) := by
   induction toErase generalizing l with
   | nil =>
     simp [eraseList, containsKey]
@@ -5366,7 +5366,7 @@ theorem eraseList_perm_filter_containsKey [BEq α] [EquivBEq α] (l toErase : Li
       simp only [List.filter_cons_of_pos, List.perm_cons]
       apply t_ih
   | cons kv tl ih =>
-    simp only [eraseList]
+    simp only [List.map_cons, eraseList]
     apply Perm.trans
     · apply ih
       · apply DistinctKeys.eraseKey hl
@@ -5416,7 +5416,7 @@ theorem eraseList_perm_filter_containsKey [BEq α] [EquivBEq α] (l toErase : Li
         · exact hl
         · apply DistinctKeys.eraseKey hl
 
-theorem eraseList_perm_of_perm_first [BEq α] [EquivBEq α] {l1 l2 toErase : List ((a : α) × β a)}
+theorem eraseList_perm_of_perm_first [BEq α] [EquivBEq α] {l1 l2 : List ((a : α) × β a)} {toErase : List α}
     (h : Perm l1 l2) (distinct : DistinctKeys l1) :
     Perm (eraseList l1 toErase) (eraseList l2 toErase) := by
   induction toErase generalizing l1 l2 with
